recursors_api/UnitTests/t11_strpos_uparams.v
@@ -2,7 +2,9 @@ From MetaCoq.Utils Require Import utils.
 From MetaCoq.Template Require Import All.
 
 From RecAPI Require Import unit_tests.
+From RecAPI Require Import nesting_param.
 
+MetaCoq Run (tmPrint "Test t11 strpos uprams").
 
 (* [false]  *)
 (* Basic *)
@@ -10,8 +12,9 @@ Inductive non_strpos (A : Type) : Type :=
 | nstrpos1 : non_strpos A
 | nstrpos2 : (A -> non_strpos A) -> non_strpos A.
 
-Redirect "recursors_api/unit_tests/tests/11_01_non_strpos_coq" MetaCoq Run (print_rec "non_strpos" ).
-Redirect "recursors_api/unit_tests/tests/11_01_non_strpos_gen" MetaCoq Run (gen_rec [] non_strpos).
+MetaCoq Run (tmPrint "Test non_strpos").
+Redirect "recursors_api/UnitTests/tests/11_01_non_strpos_coq" MetaCoq Run (print_rec "non_strpos" ).
+Redirect "recursors_api/UnitTests/tests/11_01_non_strpos_gen" MetaCoq Run (gen_rec Ep non_strpos).
 
 (* [false, false] *)
 (* Alllowed nesting *)
@@ -19,16 +22,18 @@ Inductive non_strpos2 (A B : Type) : Type :=
 | nstrpos21 : non_strpos2 A B
 | nstrpos22 : (A -> (list B) -> non_strpos2 A B) -> non_strpos2 A B.
 
-Redirect "recursors_api/unit_tests/tests/11_02_non_strpos_coq" MetaCoq Run (print_rec "non_strpos2" ).
-Redirect "recursors_api/unit_tests/tests/11_02_non_strpos_gen" MetaCoq Run (gen_rec [] non_strpos2).
+MetaCoq Run (tmPrint "Test non_strpos2").
+Redirect "recursors_api/UnitTests/tests/11_02_non_strpos_coq" MetaCoq Run (print_rec "non_strpos2" ).
+Redirect "recursors_api/UnitTests/tests/11_02_non_strpos_gen" MetaCoq Run (gen_rec Ep non_strpos2).
 
 (* [false, false] *)
 Inductive non_strpos3 (A B : Type) : Type :=
 | nstrpos31 : B -> non_strpos3 A B
 | nstrpos32 : (A -> B -> A * B -> False) -> non_strpos3 A B.
 
-Redirect "recursors_api/unit_tests/tests/11_03_non_strpos_coq" MetaCoq Run (print_rec "non_strpos3" ).
-Redirect "recursors_api/unit_tests/tests/11_03_non_strpos_gen" MetaCoq Run (gen_rec [] non_strpos3).
+MetaCoq Run (tmPrint "Test non_strpos3").
+Redirect "recursors_api/UnitTests/tests/11_03_non_strpos_coq" MetaCoq Run (print_rec "non_strpos3" ).
+Redirect "recursors_api/UnitTests/tests/11_03_non_strpos_gen" MetaCoq Run (gen_rec Ep non_strpos3).
 
 (* [false, true, true] *)
 (* Allowed nesting but left *)
@@ -36,8 +41,9 @@ Inductive non_strpos4 (A B C : Type) : Type :=
 | nstrpos41 : A -> non_strpos4 A B C
 | nstrpos42 : C -> (list A -> False) -> non_strpos4 A B C.
 
-Redirect "recursors_api/unit_tests/tests/11_04_non_strpos_coq" MetaCoq Run (print_rec "non_strpos4" ).
-Redirect "recursors_api/unit_tests/tests/11_04_non_strpos_gen" MetaCoq Run (gen_rec [] non_strpos4).
+MetaCoq Run (tmPrint "Test non_strpos4").
+Redirect "recursors_api/UnitTests/tests/11_04_non_strpos_coq" MetaCoq Run (print_rec "non_strpos4" ).
+Redirect "recursors_api/UnitTests/tests/11_04_non_strpos_gen" MetaCoq Run (gen_rec Ep non_strpos4).
 
 (* [true, true]  *)
 (* Left allowed + nesting *)
@@ -45,39 +51,38 @@ Inductive non_strpos5 (A B : Type) : Type :=
 | nstrpos51 : A -> non_strpos5 A B
 | nstrpos52 : (nat -> A) -> non_strpos5 A B.
 
-Redirect "recursors_api/unit_tests/tests/11_05_non_strpos_coq" MetaCoq Run (print_rec "non_strpos5" ).
-Redirect "recursors_api/unit_tests/tests/11_05_non_strpos_gen" MetaCoq Run (gen_rec [] non_strpos5).
+MetaCoq Run (tmPrint "Test non_strpos5").
+Redirect "recursors_api/UnitTests/tests/11_05_non_strpos_coq" MetaCoq Run (print_rec "non_strpos5" ).
+Redirect "recursors_api/UnitTests/tests/11_05_non_strpos_gen" MetaCoq Run (gen_rec Ep non_strpos5).
 
 (* [false, false, false] *)
 (* Application but not nesting *)
-(* WARNING BUGS *)
 Inductive non_strpos6 (A : Type) (f : nat -> Type -> Type) (n : nat) : Type :=
 | nstrpos61 : n = 0 -> non_strpos6 A f n
 | nstrpos62 : (nat -> f n A) -> non_strpos6 A f n.
 
-Redirect "recursors_api/unit_tests/tests/11_06_non_strpos_coq" MetaCoq Run (print_rec "non_strpos6" ).
-Redirect "recursors_api/unit_tests/tests/11_06_non_strpos_gen" MetaCoq Run (gen_rec [] non_strpos6).
+MetaCoq Run (tmPrint "Test non_strpos6").
+Redirect "recursors_api/UnitTests/tests/11_06_non_strpos_coq" MetaCoq Run (print_rec "non_strpos6" ).
+Redirect "recursors_api/UnitTests/tests/11_06_non_strpos_gen" MetaCoq Run (gen_rec Ep non_strpos6).
 
 (* [true, false, false] *)
-(* Nesting not allowed *)
+(* Nesting not allowed       *)
 Inductive non_strpos7 (A B : Type) (n : nat) : Type :=
 | nstrpos71 : n = 0 -> non_strpos7 A B n
-| nstrpos72 : A -> non_strpos B -> non_strpos7 A B n.
+| nstrpos72 : A -> Nstrpos B -> non_strpos7 A B n.
 
-Redirect "recursors_api/unit_tests/tests/11_07_non_strpos_coq" MetaCoq Run (print_rec "non_strpos7" ).
-Redirect "recursors_api/unit_tests/tests/11_07_non_strpos_gen" MetaCoq Run (gen_rec [] non_strpos7).
+MetaCoq Run (tmPrint "Test non_strpos7").
+Redirect "recursors_api/UnitTests/tests/11_07_non_strpos_coq" MetaCoq Run (print_rec "non_strpos7" ).
+Redirect "recursors_api/UnitTests/tests/11_07_non_strpos_gen" MetaCoq Run (gen_rec Ep non_strpos7).
 
 (* [true, true, false] *)
 Inductive non_strpos8 (A B : Type) (n : nat) : Type :=
 | nstrpos81 : n = 0 -> non_strpos8 A B n
 | nstrpos82 : A -> list B -> non_strpos8 A B n.
 
-Redirect "recursors_api/unit_tests/tests/11_08_non_strpos_coq" MetaCoq Run (print_rec "non_strpos8" ).
-Redirect "recursors_api/unit_tests/tests/11_08_non_strpos_gen" MetaCoq Run (gen_rec [] non_strpos8).
-
-Inductive mixed1 (A B C : Type) : Type :=
-| mc11 : mixed1 A B C
-| mc12 : mixed1 A nat C -> mixed1 A B C.
+MetaCoq Run (tmPrint "Test non_strpos8").
+Redirect "recursors_api/UnitTests/tests/11_08_non_strpos_coq" MetaCoq Run (print_rec "non_strpos8" ).
+Redirect "recursors_api/UnitTests/tests/11_08_non_strpos_gen" MetaCoq Run (gen_rec Ep non_strpos8).
 
 (* [false, true, false] *)
 (* Nesting on a nuparams => not allowed *)
@@ -85,5 +90,11 @@ Inductive non_strpos9 (A B : Type) (n : nat) : Type :=
 | nstrpos91 : n = 0 -> non_strpos9 A B n
 | nstrpos92 : A -> mixed1 B A nat -> non_strpos9 A B n.
 
-Redirect "recursors_api/unit_tests/tests/11_09_non_strpos_coq" MetaCoq Run (print_rec "non_strpos9" ).
-Redirect "recursors_api/unit_tests/tests/11_09_non_strpos_gen" MetaCoq Run (gen_rec [] non_strpos9).
+MetaCoq Run (tmPrint "Test non_strpos9").
+Redirect "recursors_api/UnitTests/tests/11_09_non_strpos_coq" MetaCoq Run (print_rec "non_strpos9" ).
+Redirect "recursors_api/UnitTests/tests/11_09_non_strpos_gen" MetaCoq Run (gen_rec Ep non_strpos9).
+
+(* Nesting on indices is not allowed *)
+MetaCoq Run (tmPrint "Test eq").
+Redirect "recursors_api/UnitTests/tests/11_10_eq_coq" MetaCoq Run (print_rec "eq" ).
+Redirect "recursors_api/UnitTests/tests/11_10_eq_gen" MetaCoq Run (gen_rec Ep (@eq)).
