recursors_api/CustomParam/fundamental_theorem_term.v
@@ -15,7 +15,7 @@ Section CustomParam.
   Context (knamep : kername).
   Context (U : output_univ).
   Context (E : global_env).
-  Context (Ep : env_param).
+  Context (Ep : param_env).
 
   Section GetRecCall.
 
