recursors_api/Preprocess/strictly_positive_uniform_parameters.v
@@ -1,5 +1,4 @@
 From RecAPI Require Import api_debruijn.
-From RecAPI Require Import uniform_parameters.
 
 
 (* 0. Aux functions *)
@@ -48,12 +47,11 @@ Section CustomParam.
 
   Context (kname : kername).
   Context (mdecl : mutual_inductive_body).
+  Context (nb_uparams : nat).
   Context (E : global_env).
-  (* Context (Ep : env_param). *)
+  Context (Ep : param_env).
 
   (* 1. Default value and bin op *)
-  Definition nb_uparams := preprocess_uparams kname mdecl E.
-
   Definition default_value : list bool :=
   let uparams := firstn nb_uparams (rev mdecl.(ind_params)) in
   let isType decl := match reduce_full E init_state decl.(decl_type)
@@ -68,149 +66,101 @@ Section CustomParam.
   Notation "l1 &&l l2" := (and_list l1 l2) (at level 50).
 
 
-  (* 2. Compute strict pos for an arg *)
-  Context (id_params : list ident).
-
   Definition get_rel (ty : term) : nat :=
     match ty with
     | tRel i => i
     | _ => 404
     end.
 
+  (* 2. Compute strict pos for an arg *)
+Section CheckArg.
+  Context (id_inds   : list ident).
+  Context (id_uparams : list ident).
+  Context (id_nuparams : list ident).
 
   Definition check_not_free (ty : term) (s : state) : list bool :=
     map (fun pos => noccur_between pos 1 ty)
-        (map get_rel (get_terms id_params s)).
+        (map get_rel (get_terms id_uparams s)).
 
-
-  Context (preprocess_strpos : kername -> mutual_inductive_body -> global_env -> list bool).
-
-
-  (* main functions *)
   Fixpoint preprocess_strpos_arg (ty : term) (s : state) {struct ty} : list bool :=
     let (hd, iargs) := decompose_app ty in
     match hd with
-    (* 1. If it an iterated product *)
+    (* 1. If it is an product check that id does not appear left of the arrow, and check the right side *)
     | tProd an A B => (check_not_free A s) &&l
                       (let* _ s <- add_old_var (Some "local") (mkdecl an None A) s in
                        preprocess_strpos_arg B s)
-    (* 2. ? *)
-    | tRel i => fold_right and_list default_value (map (fun X => check_not_free X s) iargs)
-    (* 3. If it an inductive type *)
+    (* 2. If it is a let in, store and check the remaining of the term *)
+    | tLetIn an A db B => let* _ s <- add_old_var (Some "local") (mkdecl an None A) s in
+                          preprocess_strpos_arg (reduce_lets s B) s
+    (* 3. If it is variable:  *)
+    | tRel n => if check_ids n id_inds s
+                (* 3.1 If it is the inductive type being defined, then nothing to check *)
+                then default_value
+                (* 3.2 Otherwise, check the arguments  *)
+                else fold_right and_list default_value (map (fun X => check_not_free X s) iargs)
+    (* 3. If it is nested *)
     | tInd (mkInd kname_indb pos_indb) _ =>
-        (* 3.1 If it is the current one *)
-        if eqb kname kname_indb then default_value else
+        (* Check if there is at least one argument to save computation *)
         if length iargs =? 0 then default_value else
-        (* 3.2 If it is nested get the mdecl *)
-        match TemplateLookup.lookup_minductive E kname_indb with
-        | None => default_value
-        | Some mdecl_indb =>
-          (* 3.2.1 Check which uparams are nestable *)
-          let nestable := preprocess_strpos kname_indb mdecl_indb E in
-          let nb_uparams_indb := length nestable in
-          let uparams_indb := firstn nb_uparams_indb iargs in
-          let nuparams_indices_indb := skipn nb_uparams_indb iargs in
-          (* 3.2.2 Check the uparams are strictly pos *)
-          let strpos_uparams_val := map2 (fun (b : bool) X =>
-            if b then preprocess_strpos_arg X s else check_not_free X s)
-                  nestable uparams_indb in
-          let strpos_uparams := fold_right and_list default_value strpos_uparams_val in
-          (* 3.2.3 Check it does not appear in uparams and indices *)
-          let strpos_nuparams_indices_val := map (fun X => check_not_free X s) nuparams_indices_indb in
-          let strpos_nuparams_indices := fold_right and_list default_value strpos_nuparams_indices_val in
-          (* Return *)
-          strpos_uparams &&l strpos_nuparams_indices
+        match find (fun x => eq_constant kname_indb x.(ep_kname)) Ep with
+        | Some (mk_one_param_env _ nb_uparams_indb nestable _ _) =>
+            (* Retrieve the instantiation *)
+            let uparams_inst := firstn nb_uparams_indb iargs in
+            let nuparams_indices_inst := skipn nb_uparams_indb iargs in
+            (* 3.1 For each uparams_inst:
+                - if you can nest on it => check for strict positivity in the instantiation
+                - if you can not => check if they appear in it *)
+            let strpos_uparams := fold_right (fun ' (b, X) t =>
+                if (b : bool) then preprocess_strpos_arg X s &&l t else check_not_free X s)
+              default_value (combine nestable uparams_inst) in
+            (* 3.2 Check they do not appear in the instantiation of nuparams or indices *)
+              let free_nuparams_indices := fold_right (fun X t => check_not_free X s &&l t)
+                                              default_value nuparams_indices_inst in
+            (* 3.3 Check they do not appear in the type of a varibale in the nuparams or indices *)
+            strpos_uparams &&l free_nuparams_indices
+        | None => all_false
         end
-    | _ => check_not_free ty s
+    | _ => default_value
     end.
 
-End CustomParam.
+
+  (* Check the uparams does not appear in the types *)
+  Definition check_free_cxt : list term -> state -> list bool :=
+    fun lty s =>
+    fold_right (fun X t => check_not_free X s &&l t)
+      default_value lty.
+
+End CheckArg.
 
 
 (* 3. Compute the number of uniform parameters of an inductive type *)
-Fixpoint preprocess_strpos (kname : kername) (mdecl : mutual_inductive_body) (E : global_env) {struct kname} : list bool :=
-  let nb_uparams := nb_params mdecl in
-  let default_value := default_value kname mdecl E in
+Definition preprocess_strpos : list bool :=
   (* add inds *)
   let s := add_mdecl kname nb_uparams mdecl init_state in
-  let* s <- replace_ind kname s in
-  (* add params *)
-  let* id_params s <- add_old_context (Some "params") (get_params kname s) s in
-  (* compute fct rec  *)
-  let fct := preprocess_strpos_arg kname mdecl E id_params preprocess_strpos in
-  check_ctors_by_arg and_list default_value E fct (get_all_args kname s) s.
+  let* id_inds s <- add_inds (get_mdecl kname s) s in
+  let* _ id_uparams _ s  <- add_old_context (Some "uparams") (get_uparams kname s) s in
+  let* _ id_nuparams _ s <- add_old_context (Some "nparams") (get_nuparams kname s) s in
+  (* 1. Check strict positivity in the arguments *)
+  (check_ctors_by_arg and_list default_value E (preprocess_strpos_arg id_inds id_uparams)
+    (get_all_args kname s) s)
+  (* Check the uparams does not appear in the types of the non uniform parameters *)
+  &&l (check_free_cxt id_uparams (map decl_type (get_nuparams kname s)) s)
+  (* Check the uparams does not appear in the types of the indices *)
+  &&l (check_free_cxt id_uparams (fold_right (fun indb t => (map decl_type indb.(ind_indices)) ++ t)
+                                    [] mdecl.(ind_bodies)) s).
 
 
+(* 4. Debug function *)
+Definition debug_preprocess_strpos : list (list (list bool)) :=
+  (* add inds *)
+  let s := add_mdecl kname nb_uparams mdecl init_state in
+  let* id_inds s <- add_inds (get_mdecl kname s) s in
+  let* _ id_uparams _ s  <- add_old_context (Some "uparams") (get_uparams kname s) s in
+  let* _ id_nuparams _ s <- add_old_context (Some "nparams") (get_nuparams kname s) s in
+  debug_check_ctors_by_arg E (preprocess_strpos_arg id_inds id_uparams) (get_all_args kname s) s
+  ++ [[(check_free_cxt id_uparams (map decl_type (get_nuparams kname s)) s)]]
+  ++ [[(check_free_cxt id_uparams (fold_right (fun indb t => (map decl_type indb.(ind_indices)) ++ t)
+                                  [] mdecl.(ind_bodies)) s)]].
 
 
-
-
-
-
-
-
-(* 4. Debug functions *)
-Inductive RoseTree (A : Type) : Type :=
-| leaf : A -> RoseTree A
-| leaf_left_tProd : A -> RoseTree A
-| node_tProd : list (RoseTree A) -> RoseTree A
-| node_nested : list (RoseTree A) -> RoseTree A.
-
-Arguments leaf {_} _.
-Arguments leaf_left_tProd {_} _.
-Arguments node_tProd {_} _.
-Arguments node_nested {_} _.
-
-(*
-Fixpoint debug_preprocess_strpos_arg (ty : term) (s : state) {struct ty} : RoseTree (state * list bool) :=
-  let (hd, iargs) := decompose_app ty in
-  match hd with
-  | tProd an A B => node_tProd [
-                    leaf_left_tProd (s , check_not_free A s) ;
-                    let s' := add_old_var (Some "local") (mkdecl an None A) s
-                    in debug_preprocess_strpos_arg B s']
-  | tRel i => leaf ([], default_value)
-  | tInd (mkInd kname_indb pos_indb) _ =>
-      if eqb kname kname_indb
-      then leaf ([], default_value)
-      else (* get mdecl associated to indb *)
-        let opt_mdecl_indb := get_mdecl_from_env kname_indb E in
-        match opt_mdecl_indb with
-        | None => leaf ([], default_value)
-        | Some mdecl_indb =>
-          (* get uparams and the rest *)
-          let nb_block_indb := length mdecl_indb.(ind_bodies) in
-          let nb_uparams_indb := preprocess_uparams kname_indb mdecl_indb E in
-          let uparams := map (lift0 1) (firstn nb_uparams_indb iargs) in
-          let indices := map (lift0 nb_block_indb) (skipn nb_uparams_indb iargs) in
-          (* update env with ind  *)
-          let s := replace_ind kname_indb mdecl_indb s in
-          (* update env with uparams and subst *)
-          let (uparams_cxt, nuparams_cxt) := split_params nb_uparams_indb mdecl_indb in
-          let s := add_replace_context (kname_to_opt "UPARAMS" kname_indb) uparams_cxt uparams s in
-          let s := add_old_context (kname_to_opt "NUPARAMS" kname_indb) [] s in
-          (* get the args and subst *)
-          (* let args := map (weaken_context s) (get_args mdecl_indb) in *)
-          let args := (get_args mdecl_indb) in
-          (* Check it does not appear in the body of cst *)
-          if nb_uparams_indb =? 0 then leaf ([], default_value) else (* for perf *)
-          node_nested (@check_ctors_by_arg (list (RoseTree (state * (list bool)))) (fun x y => app x y) [] E kname_indb (fun kname tm s => [debug_preprocess_strpos_arg kname tm s]) args s)
-          (* Check if does not appear in nuparams and indices *)
-          (* leaf (repeat false nb_uparams) *)
-          (* default_value *)
-        end
-  | _ => leaf ([], check_not_free hd s)
-  end.
-  *)
-
-  Fixpoint debug_preprocess_strpos (kname : kername) (mdecl : mutual_inductive_body) (E : global_env) {struct kname} : _ :=
-    let nb_uparams := nb_params mdecl in
-    let default_value := default_value kname mdecl E in
-    (* add inds *)
-    let s := add_mdecl kname nb_uparams mdecl init_state in
-    let* s <- replace_ind kname s in
-    (* add params *)
-    let* id_params s <- add_old_context (Some "params") (get_params kname s) s in
-    (* compute fct rec  *)
-    let fct := preprocess_strpos_arg kname mdecl E id_params preprocess_strpos in
-    debug_check_ctors_by_arg E fct (get_all_args kname s) s.
+End CustomParam.
