recursors_api/UnitTests/t07_nested_types.v
@@ -29,7 +29,7 @@ Inductive RoseTree_param1 A (PA : A -> Type) : RoseTree A -> Type :=
                   RoseTree_param1 A PA (RTnode A l).
 
 Redirect "recursors_api/UnitTests/tests/07_01_RoseTree_coq" MetaCoq Run (print_rec "RoseTree").
-Redirect "recursors_api/UnitTests/tests/07_01_RoseTree_gen"    MetaCoq Run (gen_rec E RoseTree).
+Redirect "recursors_api/UnitTests/tests/07_01_RoseTree_gen"    MetaCoq Run (gen_rec Ep RoseTree).
 
 Inductive PairTree A : Type :=
 | Pleaf (a : A) : PairTree A
@@ -50,7 +50,7 @@ Inductive PairTree_param1 A (PA : A -> Prop) : PairTree A -> Type :=
                   PairTree_param1 A PA (Pnode A p).
 
 Redirect "recursors_api/UnitTests/tests/07_02_PairTree_coq" MetaCoq Run (print_rec "PairTree").
-Redirect "recursors_api/UnitTests/tests/07_02_PairTree_gen"    MetaCoq Run (gen_rec E PairTree).
+Redirect "recursors_api/UnitTests/tests/07_02_PairTree_gen"    MetaCoq Run (gen_rec Ep PairTree).
 
 Inductive ArrowTree1 A : Type :=
 | ATleaf1 (a : A) : ArrowTree1 A
@@ -70,7 +70,7 @@ Inductive ArrowTree1_param1 A (PA : A -> Prop) : ArrowTree1 A -> Type :=
                    ArrowTree1_param1 A PA (ATnode1 A f).
 
 Redirect "recursors_api/UnitTests/tests/07_03_ArrowTree1_coq" MetaCoq Run (print_rec "ArrowTree1").
-Redirect "recursors_api/UnitTests/tests/07_03_ArrowTree1_gen"    MetaCoq Run (gen_rec E ArrowTree1).
+Redirect "recursors_api/UnitTests/tests/07_03_ArrowTree1_gen"    MetaCoq Run (gen_rec Ep ArrowTree1).
 
 Inductive ArrowTree2 A : Type :=
 | ATleaf2 (a : A) : ArrowTree2 A
@@ -90,7 +90,7 @@ Inductive ArrowTree2_param1 A (PA : A -> Prop) : ArrowTree2 A -> Type :=
                     ArrowTree2_param1 A PA (ATnode2 A l).
 
 Redirect "recursors_api/UnitTests/tests/07_04_ArrowTree2_coq" MetaCoq Run (print_rec "ArrowTree2").
-Redirect "recursors_api/UnitTests/tests/07_04_ArrowTree2_gen"    MetaCoq Run (gen_rec E ArrowTree2).
+Redirect "recursors_api/UnitTests/tests/07_04_ArrowTree2_gen"    MetaCoq Run (gen_rec Ep ArrowTree2).
 
 Inductive ArrowTree3 A : Type :=
 | ATleaf3 (a : A) : ArrowTree3 A
@@ -110,7 +110,7 @@ Inductive ArrowTree3_param1 A (PA : A -> Prop) : ArrowTree3 A -> Type :=
                     ArrowTree3_param1 A PA (ATnode3 A f).
 
 Redirect "recursors_api/UnitTests/tests/07_05_ArrowTree3_coq" MetaCoq Run (print_rec "ArrowTree3").
-Redirect "recursors_api/UnitTests/tests/07_05_ArrowTree3_gen"    MetaCoq Run (gen_rec E ArrowTree3).
+Redirect "recursors_api/UnitTests/tests/07_05_ArrowTree3_gen"    MetaCoq Run (gen_rec Ep ArrowTree3).
 
 (* ################################################# *)
 (* Partial nesting                                   *)
@@ -135,7 +135,7 @@ Inductive LeftTree_param1 A (PA : A -> Prop) : LeftTree A -> Type :=
                  LeftTree_param1 A PA (Lnode A p).
 
 Redirect "recursors_api/UnitTests/tests/07_06_LeftTree_coq" MetaCoq Run (print_rec "LeftTree").
-Redirect "recursors_api/UnitTests/tests/07_06_LeftTree_gen"    MetaCoq Run (gen_rec E LeftTree).
+Redirect "recursors_api/UnitTests/tests/07_06_LeftTree_gen"    MetaCoq Run (gen_rec Ep LeftTree).
 
 Inductive RightTree A : Type :=
 | Rleaf (a : A) : RightTree A
@@ -157,7 +157,7 @@ Inductive RightTree_param1 A (PA : A -> Prop) : RightTree A -> Type :=
                   RightTree_param1 A PA (Rnode A p).
 
 Redirect "recursors_api/UnitTests/tests/07_07_RightTree_coq" MetaCoq Run (print_rec "RightTree").
-Redirect "recursors_api/UnitTests/tests/07_07_RightTree_gen"    MetaCoq Run (gen_rec E RightTree).
+Redirect "recursors_api/UnitTests/tests/07_07_RightTree_gen"    MetaCoq Run (gen_rec Ep RightTree).
 
 (* ################################################# *)
 (* Nested nesting                                    *)
@@ -182,7 +182,7 @@ Inductive NestedTree_param1 A (PA : A -> Type) : NestedTree A -> Type :=
                  NestedTree_param1 A PA (Nnode A ll).
 
 Redirect "recursors_api/UnitTests/tests/07_08_NestedTree_coq" MetaCoq Run (print_rec "NestedTree").
-Redirect "recursors_api/UnitTests/tests/07_08_NestedTree_gen"    MetaCoq Run (gen_rec E NestedTree).
+Redirect "recursors_api/UnitTests/tests/07_08_NestedTree_gen"    MetaCoq Run (gen_rec Ep NestedTree).
 
 (* ################################################# *)
 (* Nesting with indices                              *)
@@ -208,7 +208,7 @@ Inductive VecTree_param1 A (PA : A -> Type) : VecTree A -> Type :=
                   VecTree_param1 A PA (VNnode A n p).
 
 Redirect "recursors_api/UnitTests/tests/07_09_VecTree_coq" MetaCoq Run (print_rec "VecTree").
-Redirect "recursors_api/UnitTests/tests/07_09_VecTree_gen"    MetaCoq Run (gen_rec E VecTree).
+Redirect "recursors_api/UnitTests/tests/07_09_VecTree_gen"    MetaCoq Run (gen_rec Ep VecTree).
 
 (* ################################################# *)
 (* Nesting when non strpos uparams                   *)
@@ -230,7 +230,7 @@ Inductive WTree_param1 A (PA : A -> Prop) : WTree A -> Type :=
                   WTree_param1 A PA (WTnode A ns).
 
 Redirect "recursors_api/UnitTests/tests/07_10_WTree_coq" MetaCoq Run (print_rec "WTree").
-(* Redirect "recursors_api/UnitTests/tests/07_10_WTree_gen"    MetaCoq Run (gen_rec E WTree). *)
+(* Redirect "recursors_api/UnitTests/tests/07_10_WTree_gen"    MetaCoq Run (gen_rec Ep WTree). *)
 
 Inductive nu_nested (A B C : Type) : Type :=
 | nu_nested_nil : A -> nu_nested A B C
@@ -268,7 +268,7 @@ Inductive tricky1_param1 A (PA : A -> Prop) : tricky1 A -> Type :=
 
 Redirect "recursors_api/UnitTests/tests/07_12_tricky1_coq" MetaCoq Run (print_rec "tricky1").
 (* BUGS ISSUE UNIVERSE LEVEL *)
-(* Redirect "recursors_api/UnitTests/tests/07_12_tricky1_gen" MetaCoq Run (gen_rec E tricky1). *)
+(* Redirect "recursors_api/UnitTests/tests/07_12_tricky1_gen" MetaCoq Run (gen_rec Ep tricky1). *)
 
 Inductive tricky2 A : Type :=
 | tricky21 : list A -> tricky2 A.
@@ -279,7 +279,7 @@ Inductive tricky2_param1 A (PA : A -> Prop) : tricky2 A -> Type :=
 
 Redirect "recursors_api/UnitTests/tests/07_13_tricky3_coq" MetaCoq Run (print_rec "tricky2").
 (* BUGS ISSUE UNIVERSE LEVEL *)
-(* Redirect "recursors_api/UnitTests/tests/07_13_tricky_gen" MetaCoq Run (gen_rec E tricky2). *)
+(* Redirect "recursors_api/UnitTests/tests/07_13_tricky_gen" MetaCoq Run (gen_rec Ep tricky2). *)
 
 Inductive tricky3 A : Type :=
 | tricky31 : A * A -> tricky3 A
@@ -293,4 +293,4 @@ Inductive tricky3_param1 A (PA : A -> Prop) : tricky3 A -> Type :=
 
 Redirect "recursors_api/UnitTests/tests/07_14_tricky3_coq" MetaCoq Run (print_rec "tricky3").
 (* BUGS ISSUE UNIVERSE LEVEL *)
-(* Redirect "recursors_api/UnitTests/tests/07_14_tricky_gen" MetaCoq Run (gen_rec E tricky3). *)
+(* Redirect "recursors_api/UnitTests/tests/07_14_tricky_gen" MetaCoq Run (gen_rec Ep tricky3). *)
