recursors_named/commons.v
@@ -7,14 +7,14 @@ Import ListNotations.
 
 
 (* Records *)
-Record one_env_param : Type := mk_one_env_param
+Record one_param_env : Type := mk_one_param_env
  { ep_kname : kername ;
    ep_body : mutual_inductive_body ;
    ep_pkname : kername ;
    ep_tkname : kername;
 }.
 
-Definition env_param := list one_env_param.
+Definition param_env := list one_param_env.
 
 Record output_univ : Type := mk_output_univ
   { out_univ  : term;
